generalize all filterMap variants to heterogeneous monads

src/Std/Data/Iterators/Consumers/Monadic/Collect.lean
@@ -34,12 +34,14 @@ This class is experimental and users of the iterator API should not explicitly d
 They can, however, assume that consumers that require an instance will work for all iterators
 provided by the standard library.
 -/
-class IteratorCollect (α : Type w) (m : Type w → Type w') {β : Type w} [Iterator α m β] where
+class IteratorCollect (α : Type w) (m : Type w → Type w') (n : Type w → Type w'')
+    {β : Type w} [Iterator α m β] where
   /--
   Maps the emitted values of an iterator using the given function and collects the results in an
   `Array`. This is an internal implementation detail. Consider using `it.map f |>.toArray` instead.
   -/
-  toArrayMapped [Finite α m] : ∀ {γ : Type w}, (β → m γ) → IterM (α := α) m β → m (Array γ)
+  toArrayMapped [Finite α m] :
+    (lift : {δ : Type w} → m δ → n δ) → {γ : Type w} → (β → n γ) → IterM (α := α) m β → n (Array γ)
 
 /--
 `IteratorCollectPartial α m` provides efficient implementations of collectors for `α`-based
@@ -49,14 +51,15 @@ This class is experimental and users of the iterator API should not explicitly d
 They can, however, assume that consumers that require an instance will work for all iterators
 provided by the standard library.
 -/
-class IteratorCollectPartial
-    (α : Type w) (m : Type w → Type w') {β : Type w} [Iterator α m β] where
+class IteratorCollectPartial (α : Type w) (m : Type w → Type w') (n : Type w → Type w'')
+    {β : Type w} [Iterator α m β] where
   /--
   Maps the emitted values of an iterator using the given function and collects the results in an
   `Array`. This is an internal implementation detail.
   Consider using `it.map f |>.allowNontermination.toArray` instead.
   -/
-  toArrayMappedPartial : ∀ {γ : Type w}, (β → m γ) → IterM (α := α) m β → m (Array γ)
+  toArrayMappedPartial :
+    (lift : {δ : Type w} → m δ → n δ) → {γ : Type w} → (β → n γ) → IterM (α := α) m β → n (Array γ)
 
 end Typeclasses
 
@@ -69,12 +72,14 @@ It iterates over an iterator and applies `f` whenever a value is emitted before 
 of `f` into an array.
 -/
 @[always_inline, inline]
-def IterM.DefaultConsumers.toArrayMapped {α : Type w} {m : Type w → Type w'} [Monad m] {β : Type w}
-    [Iterator α m β] [Finite α m] {γ : Type w} (f : β → m γ) (it : IterM (α := α) m β) : m (Array γ) :=
+def IterM.DefaultConsumers.toArrayMapped {α β : Type w} {m : Type w → Type w'}
+    {n : Type w → Type w''} [Monad n] [Iterator α m β] [Finite α m]
+    (lift : {α : Type w} → m α → n α) {γ : Type w} (f : β → n γ)
+    (it : IterM (α := α) m β) : n (Array γ) :=
   go it #[]
 where
   @[specialize]
-  go [Monad m] [Finite α m] (it : IterM (α := α) m β) a := do
+  go [Monad n] [Finite α m] (it : IterM (α := α) m β) a := letI : MonadLift m n := ⟨lift⟩; do
     match ← it.step with
     | .yield it' b _ => go it' (a.push (← f b))
     | .skip it' _ => go it' a
@@ -88,29 +93,32 @@ data structure. For certain iterators, more efficient implementations are possib
 used instead.
 -/
 @[always_inline, inline]
-def IteratorCollect.defaultImplementation {α : Type w} {m : Type w → Type w'}
-    [Monad m] [Iterator α m β] : IteratorCollect α m where
+def IteratorCollect.defaultImplementation {α β : Type w} {m : Type w → Type w'}
+    {n : Type w → Type w''} [Monad n] [Iterator α m β] [Finite α m] :
+    IteratorCollect α m n where
   toArrayMapped := IterM.DefaultConsumers.toArrayMapped
 
 /--
 Asserts that a given `IteratorCollect` instance is equal to `IteratorCollect.defaultImplementation`.
 (Even though equal, the given instance might be vastly more efficient.)
 -/
-class LawfulIteratorCollect (α : Type w) (m : Type w → Type w') [Monad m] [Iterator α m β]
-    [i : IteratorCollect α m] where
+class LawfulIteratorCollect (α : Type w) (m : Type w → Type w') (n : Type w → Type w'')
+    {β : Type w} [Monad n] [Iterator α m β] [Finite α m] [i : IteratorCollect α m n] where
   lawful : i = .defaultImplementation
 
-theorem LawfulIteratorCollect.toArrayMapped_eq {α β γ : Type w} {m : Type w → Type w'} [Monad m]
-    [Iterator α m β] [Finite α m] [IteratorCollect α m] [hl : LawfulIteratorCollect α m]
-    {f : β → m γ} {it : IterM (α := α) m β} :
-    IteratorCollect.toArrayMapped f it = IterM.DefaultConsumers.toArrayMapped f it := by
+theorem LawfulIteratorCollect.toArrayMapped_eq {α β γ : Type w} {m : Type w → Type w'}
+    {n : Type w → Type w''} [Monad n] [Iterator α m β] [Finite α m] [IteratorCollect α m n]
+    [hl : LawfulIteratorCollect α m n] {lift : {δ : Type w} → m δ → n δ}
+    {f : β → n γ} {it : IterM (α := α) m β} :
+    IteratorCollect.toArrayMapped lift f it (m := m) =
+      IterM.DefaultConsumers.toArrayMapped lift f it (m := m) := by
   cases hl.lawful; rfl
 
-instance (α : Type w) (m : Type w → Type w') [Monad m] [Iterator α m β]
-    [Monad m] [Iterator α m β] [Finite α m] :
-    haveI : IteratorCollect α m := .defaultImplementation
-    LawfulIteratorCollect α m :=
-  letI : IteratorCollect α m := .defaultImplementation
+instance (α β : Type w) (m : Type w → Type w') (n : Type w → Type w'') [Monad n]
+    [Iterator α m β] [Monad m] [Iterator α m β] [Finite α m] :
+    haveI : IteratorCollect α m n := .defaultImplementation
+    LawfulIteratorCollect α m n :=
+  letI : IteratorCollect α m n := .defaultImplementation
   ⟨rfl⟩
 
 /--
@@ -120,12 +128,14 @@ It iterates over an iterator and applies `f` whenever a value is emitted before 
 of `f` into an array.
 -/
 @[always_inline, inline]
-partial def IterM.DefaultConsumers.toArrayMappedPartial {α : Type w} {m : Type w → Type w'} [Monad m] {β : Type w}
-    [Iterator α m β] {γ : Type w} (f : β → m γ) (it : IterM (α := α) m β) : m (Array γ) :=
+partial def IterM.DefaultConsumers.toArrayMappedPartial {α β : Type w} {m : Type w → Type w'}
+    {n : Type w → Type w''} [Monad n] [Iterator α m β]
+    (lift : {α : Type w} → m α → n α) {γ : Type w} (f : β → n γ)
+    (it : IterM (α := α) m β) : n (Array γ) :=
   go it #[]
 where
   @[specialize]
-  go [Monad m] (it : IterM (α := α) m β) a := do
+  go [Monad n] (it : IterM (α := α) m β) a := letI : MonadLift m n := ⟨lift⟩; do
     match ← it.step with
     | .yield it' b _ => go it' (a.push (← f b))
     | .skip it' _ => go it' a
@@ -138,8 +148,9 @@ data structure. For certain iterators, more efficient implementations are possib
 used instead.
 -/
 @[always_inline, inline]
-def IteratorCollectPartial.defaultImplementation {α : Type w} {m : Type w → Type w'}
-    [Monad m] [Iterator α m β] : IteratorCollectPartial α m where
+def IteratorCollectPartial.defaultImplementation {α β : Type w} {m : Type w → Type w'}
+    {n : Type w → Type w''} [Monad n] [Iterator α m β] :
+    IteratorCollectPartial α m n where
   toArrayMappedPartial := IterM.DefaultConsumers.toArrayMappedPartial
 
 /--
@@ -151,9 +162,10 @@ number of steps. If the iterator is not finite or such an instance is not availa
 verify the behavior of the partial variant.
 -/
 @[always_inline, inline]
-def IterM.toArray {α : Type w} {m : Type w → Type w'} {β : Type w} [Monad m]
-    [Iterator α m β] [Finite α m] [IteratorCollect α m] (it : IterM (α := α) m β) : m (Array β) :=
-  IteratorCollect.toArrayMapped pure it
+def IterM.toArray {α β : Type w} {m : Type w → Type w'} [Monad m]
+    [Iterator α m β] [Finite α m] [IteratorCollect α m m]
+    (it : IterM (α := α) m β) : m (Array β) :=
+  IteratorCollect.toArrayMapped id pure it
 
 /--
 Traverses the given iterator and stores the emitted values in an array.
@@ -163,8 +175,8 @@ its behavior. If the iterator has a `Finite` instance, consider using `IterM.toA
 -/
 @[always_inline, inline]
 def IterM.Partial.toArray {α : Type w} {m : Type w → Type w'} {β : Type w} [Monad m]
-    [Iterator α m β] (it : IterM.Partial (α := α) m β) [IteratorCollectPartial α m] : m (Array β) :=
-  IteratorCollectPartial.toArrayMappedPartial pure it.it
+    [Iterator α m β] (it : IterM.Partial (α := α) m β) [IteratorCollectPartial α m m] : m (Array β) :=
+  IteratorCollectPartial.toArrayMappedPartial id pure it.it
 
 end ToArray
 
@@ -219,7 +231,7 @@ formally verify the behavior of the partial variant.
 -/
 @[always_inline, inline]
 def IterM.toList {α : Type w} {m : Type w → Type w'} [Monad m] {β : Type w}
-    [Iterator α m β] [Finite α m] [IteratorCollect α m] (it : IterM (α := α) m β) : m (List β) :=
+    [Iterator α m β] [Finite α m] [IteratorCollect α m m] (it : IterM (α := α) m β) : m (List β) :=
   Array.toList <$> IterM.toArray it
 
 /--
@@ -231,7 +243,8 @@ its behavior. If the iterator has a `Finite` instance, consider using `IterM.toL
 -/
 @[always_inline, inline]
 def IterM.Partial.toList {α : Type w} {m : Type w → Type w'} [Monad m] {β : Type w}
-    [Iterator α m β] (it : IterM.Partial (α := α) m β) [IteratorCollectPartial α m] : m (List β) :=
+    [Iterator α m β] (it : IterM.Partial (α := α) m β) [IteratorCollectPartial α m m] :
+    m (List β) :=
   Array.toList <$> it.toArray
 
 end Std.Iterators
